stlc_arith

swotarfe_andufotions/src/StlcProp.v
@@ -193,12 +193,12 @@ Qed.
 
 (* This is ridiculous. *)
 
-Definition progress_statement:
+Definition progress_statement:=
   forall t T,
   (fun _ => None) |- t \in T ->
   (~ stuck t).
 
-Definition preservation_statement:
+Definition preservation_statement:=
   forall t t' T,
   (fun _ => None) |- t \in T ->
   t ==> t' ->
@@ -298,3 +298,320 @@ Definition preservation_statement:
 *)
 
 (* END stlc_variation7. *)
+
+End STLCProp.
+
+Module STLCArith.
+
+Inductive ty : Type :=
+  | TArrow : ty -> ty -> ty
+  | TNat : ty.
+
+Inductive tm : Type :=
+  | tvar : id -> tm
+  | tapp : tm -> tm -> tm
+  | tabs : id -> ty -> tm -> tm
+  | tnat : nat -> tm
+  | tsucc : tm -> tm
+  | tpred : tm -> tm
+  | tmult : tm -> tm -> tm
+  | tif0  : tm -> tm -> tm -> tm.
+
+(* Exercise: 4 stars (stlc_arith) *)
+
+Definition x := (Id 0).
+Definition y := (Id 1).
+Definition z := (Id 2).
+Hint Unfold x.
+Hint Unfold y.
+Hint Unfold z.
+
+Reserved Notation "'[' x ':=' s ']' t" (at level 20).
+
+Fixpoint subst (x : id) (s : tm) (t : tm) : tm :=
+  match t with
+    | tvar i   => if eq_id_dec i x then s else tvar i
+    | tapp a b => tapp ([x := s] a) ([x := s] b)
+    | tabs i tp bd => if eq_id_dec i x then tabs i tp bd
+                      else tabs i tp ([x := s] bd)
+    | tif0 c bt be => tif0 ([x := s] c) ([x := s] bt) ([x := s] be)
+    | tsucc a => tsucc ([x := s] a)
+    | tpred a => tpred ([x := s] a)
+    | tmult a b => tmult ([x := s] a) ([x := s] b)
+    | e => e
+  end
+  where "'[' x ':=' s ']' t" := (subst x s t).
+
+Inductive value : tm -> Prop :=
+  | v_abs   : forall x T t, value (tabs x T t)
+  | v_nat   : forall n, value (tnat n).
+
+Hint Constructors value.
+
+Reserved Notation "t1 '==>' t2" (at level 40).
+
+Inductive step : tm -> tm -> Prop :=
+  | ST_AppAbs : forall x T t12 v2,
+      value v2 ->
+      (tapp (tabs x T t12) v2) ==> [x := v2] t12
+  | ST_App1   : forall t1 t1' t2,
+      t1 ==> t1' ->
+      tapp t1 t2 ==> tapp t1' t2
+  | ST_App2   : forall t1 t2 t2',
+      value t1 ->
+      t2 ==> t2' ->
+      tapp t1 t2 ==> tapp t1 t2'
+  | ST_SuccNat : forall n,
+      tsucc (tnat n) ==> tnat (S n)
+  | ST_Succ : forall t t',
+      t ==> t' ->
+      tsucc t ==> tsucc t'
+  | ST_PredNat : forall n,
+      tpred (tnat n) ==> tnat (pred n)
+  | ST_Pred : forall t t',
+      t ==> t' ->
+      tpred t ==> tpred t'
+  | ST_MultNat : forall n1 n2,
+      tmult (tnat n1) (tnat n2) ==> tnat (n1 * n2)
+  | ST_Mult1 : forall t1 t1' t2,
+      t1 ==> t1' ->
+      tmult t1 t2 ==> tmult t1' t2
+  | ST_Mult2 : forall t1 t2 t2',
+      value t1 ->
+      t2 ==> t2' ->
+      tmult t1 t2 ==> tmult t1 t2'
+  | ST_If0True  : forall t e,
+      tif0 (tnat 0) t e ==> t
+  | ST_If0False : forall t e n,
+      tif0 (tnat (S n)) t e ==> e
+  | ST_If0 : forall c c' t e,
+      c ==> c' ->
+      tif0 c t e ==> tif0 c' t e
+  where "t1 '==>' t2" := (step t1 t2).
+
+Hint Constructors step.
+
+Notation multistep := (multi step).
+
+Notation "t1 '==>*' t2" := (multistep t1 t2) (at level 40).
+
+Definition context := id -> option ty.
+
+Definition pupdate { A : Type } (m : id -> option A) (x : id) (v : A) :=
+  update m x (Some v).
+
+Hint Unfold pupdate.
+
+Reserved Notation "Gamma '|-' t '\in' T" (at level 40).
+
+Inductive has_type : context -> tm -> ty -> Prop :=
+  | T_Var : forall G i T,
+      G i = Some T ->
+      G |- tvar i \in T
+  | T_Abs : forall G i T11 bd T12,
+      pupdate G i T11 |- bd \in T12 ->
+      G |- tabs i T11 bd \in TArrow T11 T12
+  | T_App : forall G a1 a2 T11 T12,
+      G |- a1 \in TArrow T11 T12 ->
+      G |- a2 \in T11 ->
+      G |- tapp a1 a2 \in T12
+  | T_Nat : forall G n,
+      G |- tnat n \in TNat
+  | T_Succ : forall G t,
+      G |- t \in TNat ->
+      G |- tsucc t \in TNat
+  | T_Pred : forall G t,
+      G |- t \in TNat ->
+      G |- tpred t \in TNat
+  | T_Mult : forall G t1 t2,
+      G |- t1 \in TNat ->
+      G |- t2 \in TNat ->
+      G |- tmult t1 t2 \in TNat
+  | T_If0 : forall G c t e T,
+      G |- c \in TNat ->
+      G |- t \in T ->
+      G |- e \in T ->
+      G |- (tif0 c t e) \in T
+  where "Gamma '|-' t '\in' T" := (has_type Gamma t T).
+
+Hint Constructors has_type.
+
+Lemma canonical_forms_nat : forall t,
+  (fun _ => None) |- t \in TNat ->
+  value t ->
+  (exists n, t = tnat n).
+Proof.
+  intros. inversion H; subst; try solve by inversion; eauto.
+Qed.
+
+Lemma canonical_forms_fun : forall t T1 T2,
+  (fun _ => None) |- t \in TArrow T1 T2 ->
+  value t ->
+  (exists x u, t = tabs x T1 u).
+Proof.
+  intros. inversion H; subst; try inversion H0; subst.
+  exists i. exists bd. trivial.
+Qed.
+
+Theorem progress : forall t T,
+  (fun _ => None) |- t \in T ->
+  value t \/ exists t', t ==> t'.
+Proof.
+  induction t; intros; auto; inversion H; subst.
+  - solve by inversion.
+  - right. destruct IHt1 with (TArrow T11 T); try assumption.
+    + destruct (canonical_forms_fun t1 T11 T) as [x [u Hu]]; subst; eauto.
+      apply IHt2 in H5. destruct H5 as [vt2 | [z Hex]]; eauto.
+    + destruct H0 as [x Hex]. eauto.
+  - right. edestruct IHt; try eassumption.
+    + destruct (canonical_forms_nat t); subst; eauto.
+    + destruct H0; eauto.
+  - right. edestruct IHt; try eassumption.
+    + destruct (canonical_forms_nat t); subst; eauto.
+    + destruct H0; eauto.
+  - right. edestruct IHt1; try eassumption.
+    + destruct (canonical_forms_nat t1); subst; eauto.
+      edestruct IHt2; try eassumption.
+      * destruct (canonical_forms_nat t2); subst; eauto.
+      * destruct H1; eauto.
+    + destruct H0; eauto.
+  - right. edestruct IHt1; try eassumption.
+    + destruct (canonical_forms_nat t1); subst; eauto.
+      destruct x0; eauto.
+    + destruct H0; eauto.
+Qed.
+
+Inductive appears_free_in : id -> tm -> Prop :=
+  | afi_var : forall x,
+      appears_free_in x (tvar x)
+  | afi_app1 : forall x t1 t2,
+      appears_free_in x t1 ->
+      appears_free_in x (tapp t1 t2)
+  | afi_app2 : forall x t1 t2,
+      appears_free_in x t2 ->
+      appears_free_in x (tapp t1 t2)
+  | afi_abs  : forall x i T t,
+      i <> x ->
+      appears_free_in x t ->
+      appears_free_in x (tabs i T t)
+  | afi_succ : forall x t,
+      appears_free_in x t ->
+      appears_free_in x (tsucc t)
+  | afi_pred : forall x t,
+      appears_free_in x t ->
+      appears_free_in x (tpred t)
+  | afi_mult1 : forall x t1 t2,
+      appears_free_in x t1 ->
+      appears_free_in x (tmult t1 t2)
+  | afi_mult2 : forall x t1 t2,
+      appears_free_in x t2 ->
+      appears_free_in x (tmult t1 t2)
+  | afi_if1 : forall x c t e,
+      appears_free_in x c ->
+      appears_free_in x (tif0 c t e)
+  | afi_if2 : forall x c t e,
+      appears_free_in x t ->
+      appears_free_in x (tif0 c t e)
+  | afi_if3 : forall x c t e,
+      appears_free_in x e ->
+      appears_free_in x (tif0 c t e)
+.
+
+Hint Constructors appears_free_in.
+
+Definition closed (t : tm) :=
+  forall x, ~ appears_free_in x t.
+
+Lemma free_in_context : forall x t T Gamma,
+  appears_free_in x t ->
+  Gamma |- t \in T ->
+  exists T', Gamma x = Some T'.
+Proof.
+  intros x t.
+  induction t; intros; inversion H0; subst; inversion H; subst; eauto.
+  - apply IHt in H6; auto.
+      destruct H6. unfold pupdate in H1. rewrite update_neq in H1; eauto.
+Qed.
+
+Corollary typable_empty__closed : forall t T,
+  (fun _ => None) |- t \in T ->
+  closed t.
+Proof.
+  unfold closed. intros. intro contra.
+  apply (free_in_context x0 t T (fun _ => None)) in H; eauto.
+  solve by inversion 2.
+Qed.
+
+Lemma context_invariance : forall G G' t T,
+  G  |- t \in T ->
+  (forall x, appears_free_in x t -> G x = G' x) ->
+  G' |- t \in T.
+Proof with eauto.
+  intros G G' t T Hin Hst.
+  generalize dependent Hst. generalize dependent G'.
+  induction Hin; intros; eauto; econstructor...
+  - rewrite Hst in H...
+  - unfold pupdate in *.
+    apply IHHin; intros. unfold update. destruct (eq_id_dec i x0); subst...
+Qed.
+
+Lemma substitution_preserves_typing : forall G x U t v T,
+  pupdate G x U   |- t \in T ->
+  (fun _ => None) |- v \in U ->
+  G |- [x := v] t \in T.
+Proof with eauto.
+  unfold pupdate.
+  intros G x U t.
+  generalize dependent U. generalize dependent x. generalize dependent G.
+  induction t; simpl; intros; inversion H; subst...
+  - destruct (eq_id_dec i x0); subst.
+    + rewrite update_eq in H3. inversion H3; subst.
+      eapply context_invariance...
+      intros.
+      apply typable_empty__closed in H0. unfold closed in H0.
+      apply H0 in H1. contradiction.
+    + rewrite update_neq in H3...
+  - unfold pupdate in *.
+    destruct (eq_id_dec i x0); subst.
+    + eapply context_invariance...
+      intros. inversion H1; subst.
+      rewrite update_neq...
+    + econstructor. unfold pupdate.
+      eapply IHt...
+      eapply context_invariance...
+      intros.
+      rewrite update_permute...
+Qed.
+
+Theorem preservation : forall t t' T,
+  (fun _ => None) |- t \in T ->
+  t ==> t' ->
+  (fun _ => None) |- t' \in T.
+Proof with eauto.
+  remember (fun _ => (None : option ty)) as G.
+  intros t t' T Ht. generalize dependent t'.
+  induction Ht; intros; subst; try solve
+    [inversion H; subst; eauto].
+  - inversion H; subst...
+    + apply substitution_preserves_typing with T11...
+      * inversion Ht1...
+Qed.
+
+Definition stuck (t : tm) : Prop :=
+  (normal_form step) t /\ ~ value t.
+
+Corollary soundness : forall t t' T,
+  (fun _ => None) |- t \in T ->
+  t ==>* t' ->
+  ~(stuck t').
+Proof.
+  intros t t' T Hhas_type Hmulti. unfold stuck.
+  intros [Hnf Hnot_val]. unfold normal_form in Hnf.
+  induction Hmulti.
+  - apply progress in Hhas_type. destruct Hhas_type; contradiction.
+  - apply preservation with (t' := y0) in Hhas_type; eauto.
+Qed.
+
+(* END stlc_arith. *)
+
+End STLCArith.
